


---

---

---

---

---



# PS 8

1.

(a)  $P(\uparrow_z) + P(\downarrow_z)$  should be 1.

$$(\psi_z) = \alpha |\uparrow_z\rangle + \beta |\downarrow_z\rangle,$$

$$\alpha = 1, \beta = -i, (\alpha^2 + \beta^2 = 37).$$

$$\therefore \text{normalization constant} = \frac{1}{\sqrt{37}},$$

$$\text{normalized state vector} = \frac{1}{\sqrt{37}} (6 |\uparrow_z\rangle - i |\downarrow_z\rangle)$$

$$(b) P(S_z = +\frac{\hbar}{2}) = \left| \frac{6}{\sqrt{37}} \right|^2 = \frac{36}{37}$$

$$P(S_z = -\frac{\hbar}{2}) = \left| \frac{-i}{\sqrt{37}} \right|^2 = \frac{1}{37}$$

$$(c) \frac{36}{37} + \frac{1}{37} = \frac{37}{37}$$

2.

(a) The classical prediction

: In a field gradient one would see one broadened continuous streak, not separate beams.

(b) Empirical result.

: The beam actually splits into two discrete spots with 50:50 ratio.  
We assume the spin  $S_z$  is quantized, not being continuous.

3.

$$|+\theta\rangle = \cos \frac{\theta}{2} |\uparrow\rangle + \sin \frac{\theta}{2} |\downarrow\rangle$$

$$|-\theta\rangle = -\sin \frac{\theta}{2} |\uparrow\rangle + \cos \frac{\theta}{2} |\downarrow\rangle$$

$$(a) \quad (i) \quad \langle +\theta_2 | +\theta_1 \rangle = \left( \cos \frac{\theta_2}{2} \langle \uparrow | + \sin \frac{\theta_2}{2} \langle \downarrow | \right) \left( \cos \frac{\theta_1}{2} | \uparrow \rangle + \sin \frac{\theta_1}{2} | \downarrow \rangle \right)$$

$$= \cos \frac{\theta_2}{2} \cos \frac{\theta_1}{2} \langle \uparrow | \uparrow \rangle + \cos \frac{\theta_2}{2} \sin \frac{\theta_1}{2} \langle \uparrow | \downarrow \rangle \\ + \sin \frac{\theta_2}{2} \cos \frac{\theta_1}{2} \langle \downarrow | \uparrow \rangle + \sin \frac{\theta_2}{2} \sin \frac{\theta_1}{2} \langle \downarrow | \downarrow \rangle$$

$$= \cos \frac{\theta_2}{2} \cdot \cos \frac{\theta_1}{2} + \sin \frac{\theta_2}{2} \cdot \sin \frac{\theta_1}{2}$$

$$= \cos \left( \frac{\theta_1}{2} - \frac{\theta_2}{2} \right) \dots$$

$$\text{Here } \theta_1 = -15^\circ,$$

$$\theta_2 = 35^\circ.$$

$$\Rightarrow \cos \left( \frac{\theta_1}{2} - \frac{\theta_2}{2} \right)$$

$$= \cos \left( \frac{\theta_2}{2} - \frac{\theta_1}{2} \right) = \cos \frac{50^\circ}{2}$$

$$= \cos 25^\circ.$$

$$\rightarrow \cos(A-B) = \operatorname{Re}(e^{i(A-B)})$$

$$= \operatorname{Re}(e^{iA} e^{-iB})$$

$$= \operatorname{Re}((\cos A + i \sin A)(\cos B - i \sin B))$$

$$= \cos A \cos B + \sin A \sin B$$

$$( \text{hint using GPT} )$$

$$(ii) \quad \langle +\theta_3 | +\theta_2 \rangle$$

$$\text{with same logic, with formula } \cos \left( \frac{\theta_3}{2} - \frac{\theta_2}{2} \right),$$

$$\Rightarrow \cos \frac{55^\circ}{2} = \cos 27.5^\circ$$

$$P(+\theta_3 | +\theta_1) = |\langle +\theta_2 | +\theta_1 \rangle|^2 |\langle +\theta_3 | +\theta_2 \rangle|^2$$

$$= \cos^2 25^\circ \times \cos^2 27.5^\circ \simeq 0.646$$

(b)

$$P(-\theta_3 | +\theta_1) = \underbrace{|\langle +\theta_2 | +\theta_1 \rangle|^2}_{\cos^2 25^\circ} \underbrace{|\langle -\theta_3 | +\theta_2 \rangle|^2}_{\sin^2 27.5^\circ} \Rightarrow \cos^2 25^\circ \times \sin^2 27.5^\circ \simeq 0.175$$

$$\left| \left( -\sin \frac{\theta_3}{2} \langle \uparrow | + \cos \frac{\theta_3}{2} \langle \downarrow | \right) \left( \cos \frac{\theta_2}{2} | \uparrow \rangle + \sin \frac{\theta_2}{2} | \downarrow \rangle \right) \right|^2$$

$$= \left| -\sin \frac{\theta_3}{2} \cos \frac{\theta_2}{2} + \cos \frac{\theta_3}{2} \sin \frac{\theta_2}{2} \right|^2$$

$$= \left| \sin \left( \frac{\theta_2}{2} - \frac{\theta_3}{2} \right) \right|^2 \dots \rightarrow$$

$$= \sin^2 27.5^\circ$$

$$\sin(A-B) = \operatorname{Im}(e^{i(A-B)}) = \operatorname{Im}(e^{iA} \cdot e^{-iB}) \\ \operatorname{Im}((\cos A + i \sin A)(\cos B - i \sin B)) \\ = -\cos A \sin B + \sin A \cos B$$

(c) It is because the particles that are  $|-\theta_1\rangle$  are neglected.

$|-\theta_1\rangle$  is neglectable as  $|+\theta_1\rangle$  is given as the scoring state, but once the beam reaches the second analyzer it neglects the particles that go to  $|-\theta_2\rangle$  and the rest goes on to the third analyzer.

4.

$$P(t_3|t_1) = \underbrace{P(t_2|t_1)}_{(1)} \underbrace{P(t_3|t_2)}_{(2)} = \frac{3}{8}$$

$$(1) |\langle +\theta_2 | +\theta_1 \rangle|^2, \theta_2 = 90^\circ, \theta_1 = 30^\circ$$

$$= |\cos(\frac{\theta_2 - \theta_1}{2})|^2 = |\cos 30^\circ|^2 = \frac{3}{4}.$$

$$(2) |\langle +\theta_3 | +\theta_2 \rangle|^2, \theta_3 = 0^\circ, \theta_2 = 90^\circ$$

$$= |\cos(\frac{\theta_2 - \theta_3}{2})|^2 = |\cos 45^\circ|^2 = \frac{1}{2}.$$

$$\left. \begin{matrix} (1) \\ (2) \end{matrix} \right\} \left( \frac{3}{8} \right)$$

5.

$$|\psi\rangle = \frac{1}{\sqrt{2}} (|\uparrow_z \uparrow_z\rangle + |\downarrow_z \downarrow_z\rangle)$$

(a)  $|\uparrow_{z=0}\rangle$ , 100% (= probability: 1)

Spin is in an entangled state and we already measured  $|\uparrow_{z=0}\rangle$  for A.

(b)  $|\uparrow_{z=0}\rangle$ , for the entanglement, after z-measurement,  $P(\uparrow) = \frac{1}{4}$

$$|\uparrow_{z=0}\rangle = \cos 60^\circ |\uparrow_z\rangle + \sin 60^\circ |\downarrow_z\rangle$$

$$= \frac{1}{2} |\uparrow_z\rangle + \frac{\sqrt{3}}{2} |\downarrow_z\rangle$$

(c) When both analyzers are aligned, entangled state brings perfect correlation.  
But when there is misalignment by angle  $\theta$ , the transition probability is  $\cos^2(\frac{\theta}{2})$

(I could not find the slide we looked through last week on Canvas.)